x86/RealAsm.v
@@ -39,7 +39,7 @@ Section WITHGE.
       Next (nextinstr (rs#rd <- sp) sz) m
     | Pcall_s id sg =>
       let sp := Val.offset_ptr (rs RSP) (Ptrofs.neg (Ptrofs.repr (size_chunk Mptr))) in
-      match maybe_storev Mptr m sp (Val.offset_ptr rs#PC sz) with
+      match Mem.storev Mptr m sp (Val.offset_ptr rs#PC sz) with
       | None => Stuck
       | Some m2 =>
         Next (rs#RA <- (Val.offset_ptr rs#PC sz)
@@ -48,7 +48,7 @@ Section WITHGE.
       end
     | Pcall_r r sg =>
       let sp := Val.offset_ptr (rs RSP) (Ptrofs.neg (Ptrofs.repr (size_chunk Mptr))) in
-      match maybe_storev Mptr m sp (Val.offset_ptr rs#PC sz) with
+      match Mem.storev Mptr m sp (Val.offset_ptr rs#PC sz) with
       | None => Stuck
       | Some m2 =>
         Next (rs#RA <- (Val.offset_ptr rs#PC sz)
@@ -114,7 +114,7 @@ End WITHGE.
         (MALLOC: Mem.alloc (Mem.push_new_stage m) 0 (Mem.stack_limit) = (m1,bstack))
         (MDROP: Mem.drop_perm m1 bstack 0 (Mem.stack_limit) Writable = Some m2)
         (MRSB: Mem.record_stack_blocks m2 (make_singleton_frame_adt' bstack frame_info_mono 0) = Some m3)
-        (STORE_RETADDR: maybe_storev Mptr m3 (Vptr bstack (Ptrofs.repr (Mem.stack_limit - size_chunk Mptr))) Vnullptr = Some m4),
+        (STORE_RETADDR: Mem.storev Mptr m3 (Vptr bstack (Ptrofs.repr (Mem.stack_limit - size_chunk Mptr))) Vnullptr = Some m4),
         let ge := Genv.globalenv prog in
         let rs0 :=
             rs # PC <- (Genv.symbol_address ge prog.(prog_main) Ptrofs.zero)
